progress?

memset_arm_proofs.v
@@ -67,3 +67,240 @@ Theorem memset_ret :
   eapply noassign_prog_same; [|eassumption].
   prove_noassign.
 Qed.
+
+Definition memfilled (m:addr->N) (s:addr) (c:N) n :=
+  forall i, i < n -> m (s⊕i) = c.
+
+Definition memset_bytedup b :=
+  let c := b mod (2 ^ 8)
+  in c .| c<<8 .| c<<16 .| c<<24.
+
+Definition memset_invs (s:addr) (c:N) n (a:addr) (st:store) :=
+  let common_inv :=
+      exists r1 r2 r3 prog m,
+        st V_MEM32 = Ⓜm
+        /\ st R_R0 = Ⓓs
+        /\ st R_R1 = Ⓓr1
+        /\ st R_R2 = Ⓓr2
+        /\ st R_R3 = Ⓓr3
+        /\ r3 = s ⊕ prog
+        /\ c = r1 mod (2^8)
+        /\ Ⓓ(s ⊕ n) = Ⓓ(r3 ⊕ r2)
+        /\ memfilled m s c prog
+  in match a with
+     | 0 => Some (exists m ci,
+                     st V_MEM32 = Ⓜm
+                     /\ st R_R0 = Ⓓs
+                     /\ st R_R1 = Ⓓci
+                     /\ st R_R2 = Ⓓn
+                     /\ c = ci mod (2^8))
+     (* | 4 => Some (st R_R2 = Ⓓn /\ common_inv) *)
+     | 12 => Some common_inv
+     | 44 => Some (st R_R1 = Ⓓ(memset_bytedup c)
+                   /\ st R_R1 = st R_R12
+                   /\ common_inv)
+     | 84 => Some common_inv
+     | _ => None
+     end.
+
+Definition memset_post s c n (_:exit) (st:store) :=
+  exists m, st V_MEM32 = Ⓜm /\ st R_R0 = Ⓓs /\ memfilled m s c n.
+
+Definition memset_invset s c n :=
+  invs (memset_invs s c n) (memset_post s c n).
+
+Theorem mod_greater (n d1 d2:N) :
+  d1 ≠ 0 -> d1 <= d2 -> (n mod d1) mod d2 = n mod d1.
+  intros.
+  apply N.mod_small.
+  eapply N.lt_le_trans; eauto.
+  apply N.mod_upper_bound.
+  exact H.
+Qed.
+
+Theorem mod_same (n d:N) : d ≠ 0 -> (n mod d) mod d = n mod d.
+  intros.
+  apply mod_greater; auto.
+  apply N.le_refl.
+Qed.
+
+Theorem strlen_partial_correctness:
+  forall st lr s ci c n q st' x m
+         (MDL0: models armtypctx st)
+         (LR0: st R_LR = Ⓓlr) (MEM0: st V_MEM32 = Ⓜm)
+         (R0: st R_R0 = Ⓓs) (R1: st R_R1 = Ⓓci) (R2: st R_R2 = Ⓓn)
+         (C: c = ci mod 2^8)
+         (RET: memset_arm st lr = None)
+         (XP0: exec_prog fh memset_arm 0 st q st' x),
+    trueif_inv (memset_invset s c n memset_arm x st').
+  intros.
+  eapply prove_invs.
+  exact XP0.
+  simpl.
+  eauto 7.
+  intros.
+  shelve_cases 32 PRE. Unshelve.
+
+  Local Ltac step := time arm_step.
+  step. step. step.
+  destruct PRE.
+  destruct H.
+  intuition.
+  rewrite H0,H,H1,H2,H4.
+  exists x1.
+  exists n.
+  exists s.
+  exists 0.
+  exists x0.
+  intuition.
+  rewrite N.add_0_r.
+  (* admitting s=s mod _ *)
+  admit.
+  unfold memfilled.
+  intros.
+  destruct i; inversion H3.
+  destruct PRE.
+  destruct H.
+  intuition.
+  rewrite H,H0,H1,H2.
+  exists x1,n,s,0,x0.
+  intuition.
+  (* admitting s=s mod _ *)
+  admit.
+  unfold memfilled.
+  intros.
+  destruct i; inversion H3.
+
+  destruct PRE.
+  destruct H.
+  destruct H.
+  destruct H.
+  destruct H.
+  intuition.
+  step. step. step. step.
+  inversion BC1.
+  inversion BC0.
+  step.
+  inversion BC1.
+  step.
+  step.
+  step.
+  step.
+  intuition.
+  unfold memset_bytedup.
+  Search N.modulo.
+  repeat rewrite (N.mod_small _ (2^32)).
+  rewrite H5.
+  repeat rewrite mod_same.
+  (* admitting bitwise arithmetic *)
+  admit.
+  compute.
+  intros.
+  inversion H7.
+  (* admitting more arithmetic *)
+  admit.
+  admit.
+  rewrite H.
+  econstructor.
+  exists x1,x2,x3.
+  econstructor.
+  intuition.
+  (* arith *)
+  admit.
+  repeat step.
+  do 3 econstructor.
+  exists (x3 ⊕ 1).
+  econstructor.
+  intuition.
+  rewrite H4.
+  Search N.add N.modulo.
+  repeat rewrite N.add_mod_idemp_r.
+  repeat rewrite N.add_mod_idemp_l.
+  rewrite N.add_assoc.
+  reflexivity.
+  compute.
+  intros.
+  inversion H7.
+  compute.
+  intros.
+  inversion H7.
+  rewrite H6.
+  Locate "⊖".
+  Print N.sub.
+  repeat econstructor; auto.
+  rewrite H4.
+  Search N.modulo N.add.
+  repeat rewrite N.add_mod_idemp_l.
+  repeat rewrite N.add_mod_idemp_r.
+  Search N.add eq.
+  Search (_ + _ = _ + _).
+  Locate "Ⓓ".
+  Search (VaN _ _ = VaN _ _).
+  assert (valinj : forall a b, a=b -> Ⓓa = Ⓓb).
+  intros.
+  rewrite H7.
+  reflexivity.
+  apply valinj.
+  Search N.modulo N.add.
+  repeat rewrite <- N.add_assoc.
+  rewrite N.add_1_l.
+  rewrite N.sub_1_r.
+  Search N.succ N.pred.
+  rewrite N.succ_pred.
+  Search N.add N.modulo.
+  repeat rewrite N.add_assoc.
+  simpl.
+  repeat rewrite (N.add_comm _ (N.pos (2^32))).
+  Search N.modulo N.add.
+  repeat rewrite <- N.add_assoc.
+  rewrite mod_add_l.
+  repeat rewrite N.add_mod_idemp_l.
+  rewrite N.add_assoc.
+  reflexivity.
+  Locate "≠".
+  compute. intros. inversion H7.
+  compute. intros. inversion H7.
+  rewrite N.add_comm.
+  destruct x1.
+  compute. intros. inversion H7.
+  red.
+  intros.
+  inversion H7.
+  compute. intros. inversion H7.
+  compute. intros. inversion H7.
+  compute. intros. inversion H7.
+  unfold memfilled in H8.
+  unfold memfilled.
+  intros.
+  (* dealing with store operations *)
+  destruct (N.eq_decidable i x3); subst.
+  rewrite <- H5.
+  (* this should be trivial, but isn't *)
+  admit.
+  destruct (N.lt_decidable i x3); subst.
+  rewrite <- (H8 i); auto.
+  (* again, should be trivial, isn't *)
+  admit.
+  (* arithmetic *)
+  admit.
+  (* duplicate goals from conditionals *)
+  admit.
+  admit.
+  admit.
+
+  (* main loop *)
+  admit.
+
+  (* end loop *)
+  admit.
+Abort.
+
+(* Pain points:
+   - "mod 2^32" gets attached to everything
+   - conditional instructions duplicate program proofs
+   - "s [Ⓑv := a] v" should be a, but isn't easily turned into a
+   - subtraction adds 2^32 (for modular arithmetic)
+   - Ⓓ, Ⓜ frequently require existentials to extract
+   - (related to the previous) Ⓓ, Ⓜ are secretly dynamic types
+   - It's easy to construct "impossible states" (i.e. VaN 32 2^64)
+ *)
